Test/civl/inductive-sequentialization/paxos/PaxosSeq.bpl
@@ -1,29 +1,29 @@
-atomic action {:layer 2} A_Paxos({:linear_in "perm"} rs: [Round]bool)
+atomic action {:layer 2} A_Paxos({:linear_in} ps: Set Permission)
 modifies joinedNodes, voteInfo, decision;
 refines A_Paxos' using INV;
 creates A_StartRound;
 {
   var {:pool "NumRounds"} numRounds: int;
-  assert Init(rs, decision);
+  assert Init(ps, decision);
   assume
     {:add_to_pool "Round", 0, numRounds}
     {:add_to_pool "NumRounds", numRounds}
     0 <= numRounds;
   joinedNodes := (lambda r: Round:: NoNodes());
   voteInfo := (lambda r: Round:: None());
-  call create_asyncs((lambda pa: A_StartRound :: pa->r == pa->r_lin && Round(pa->r) && pa->r <= numRounds));
+  call create_asyncs((lambda pa: A_StartRound :: AllPermissions(pa->r) == pa->r_lin && Round(pa->r) && pa->r <= numRounds));
 }
 
-atomic action {:layer 3} A_Paxos'({:linear_in "perm"} rs: [Round]bool)
+atomic action {:layer 3} A_Paxos'({:linear_in} ps: Set Permission)
 modifies decision;
 {
-  assert Init(rs, decision);
+  assert Init(ps, decision);
   havoc decision;
   assume (forall r1: Round, r2: Round :: decision[r1] is Some && decision[r2] is Some ==> decision[r1] == decision[r2]);
 }
 
 action {:layer 2}
-INV({:linear_in "perm"} rs: [Round]bool)
+INV({:linear_in} ps: Set Permission)
 creates A_StartRound, A_Propose, A_Conclude, A_Join, A_Vote;
 modifies joinedNodes, voteInfo, decision;
 {
@@ -31,7 +31,7 @@ modifies joinedNodes, voteInfo, decision;
   var {:pool "Round"} k: int;
   var {:pool "Node"} m: Node;
 
-  assert Init(rs, decision);
+  assert Init(ps, decision);
 
   havoc joinedNodes, voteInfo, decision;
 
@@ -53,21 +53,21 @@ modifies joinedNodes, voteInfo, decision;
       assume
         (forall r: Round :: r < 1 || r > k ==> voteInfo[r] is None) &&
         (forall r: Round :: r < 1 || r > k ==> decision[r] is None);
-      call create_asyncs((lambda {:pool "A_StartRound"} pa: A_StartRound :: pa->r == pa->r_lin && k < pa->r && pa->r <= numRounds));
-      call set_choice(A_StartRound(k+1, k+1));
+      call create_asyncs((lambda {:pool "A_StartRound"} pa: A_StartRound :: AllPermissions(pa->r) == pa->r_lin && k < pa->r && pa->r <= numRounds));
+      call set_choice(A_StartRound(k+1, AllPermissions(k+1)));
   } else if (*) {
       assume
         (forall r: Round :: r < 1 || r > k ==> voteInfo[r] is None) &&
         (forall r: Round :: r < 1 || r > k ==> decision[r] is None);
       assume
         {:add_to_pool "Node", m}
-        {:add_to_pool "A_Join", A_Join(k+1, numNodes, JoinPerm(k+1, numNodes))}
+        {:add_to_pool "A_Join", A_Join(k+1, numNodes, One(JoinPerm(k+1, numNodes)))}
         0 <= m && m <= numNodes;
-      call create_asyncs((lambda pa: A_StartRound :: pa->r == pa->r_lin && k+1 < pa->r && pa->r <= numRounds));
+      call create_asyncs((lambda pa: A_StartRound :: AllPermissions(pa->r) == pa->r_lin && k+1 < pa->r && pa->r <= numRounds));
       call create_async(A_Propose(k+1, ProposePermissions(k+1)));
-      call create_asyncs((lambda {:pool "A_Join"} pa: A_Join :: pa->r == k+1 && m < pa->n && pa->n <= numNodes && pa->p == JoinPerm(k+1, pa->n)));
+      call create_asyncs((lambda {:pool "A_Join"} pa: A_Join :: pa->r == k+1 && m < pa->n && pa->n <= numNodes && pa->p->val == JoinPerm(k+1, pa->n)));
       if (m == numNodes) { call set_choice(A_Propose(k+1, ProposePermissions(k+1))); }
-      else { call set_choice(A_Join(k+1, m+1, JoinPerm(k+1, m+1))); }
+      else { call set_choice(A_Join(k+1, m+1, One(JoinPerm(k+1, m+1)))); }
   } else {
       assume
         voteInfo[k+1] is Some &&
@@ -75,15 +75,15 @@ modifies joinedNodes, voteInfo, decision;
         (forall r: Round :: r < 1 || r > k ==> decision[r] is None);
       assume
         {:add_to_pool "Node", m}
-        {:add_to_pool "A_Vote", A_Vote(k+1, numNodes, voteInfo[k+1]->t->value, VotePerm(k+1, numNodes))}
-        {:add_to_pool "A_StartRound", A_StartRound(numRounds, numRounds)}
+        {:add_to_pool "A_Vote", A_Vote(k+1, numNodes, voteInfo[k+1]->t->value, One(VotePerm(k+1, numNodes)))}
+        {:add_to_pool "A_StartRound", A_StartRound(numRounds, AllPermissions(numRounds))}
         0 <= m && m <= numNodes &&
         (forall n: Node :: n < 1 || n > m ==> !voteInfo[k+1]->t->ns[n]);
-      call create_asyncs((lambda {:pool "A_StartRound"} pa: A_StartRound :: pa->r == pa->r_lin && k+1 < pa->r && pa->r <= numRounds));
-      call create_async(A_Conclude(k+1, voteInfo[k+1]->t->value, ConcludePerm(k+1)));
-      call create_asyncs((lambda {:pool "A_Vote"} pa: A_Vote :: pa->r == k+1 && m < pa->n && pa->n <= numNodes && pa->v == voteInfo[k+1]->t->value && pa->p == VotePerm(k+1, pa->n)));
-      if (m == numNodes) { call set_choice(A_Conclude(k+1, voteInfo[k+1]->t->value, ConcludePerm(k+1))); }
-      else { call set_choice(A_Vote(k+1, m+1, voteInfo[k+1]->t->value, VotePerm(k+1, m+1))); }
+      call create_asyncs((lambda {:pool "A_StartRound"} pa: A_StartRound :: AllPermissions(pa->r) == pa->r_lin && k+1 < pa->r && pa->r <= numRounds));
+      call create_async(A_Conclude(k+1, voteInfo[k+1]->t->value, One(ConcludePerm(k+1))));
+      call create_asyncs((lambda {:pool "A_Vote"} pa: A_Vote :: pa->r == k+1 && m < pa->n && pa->n <= numNodes && pa->v == voteInfo[k+1]->t->value && pa->p->val == VotePerm(k+1, pa->n)));
+      if (m == numNodes) { call set_choice(A_Conclude(k+1, voteInfo[k+1]->t->value, One(ConcludePerm(k+1)))); }
+      else { call set_choice(A_Vote(k+1, m+1, voteInfo[k+1]->t->value, One(VotePerm(k+1, m+1)))); }
   }
 
   // If there was a decision for some value, then there must have been a
